isabelle/elaborator/ElabTermCorrect.thy
@@ -2344,12 +2344,10 @@ next
       have "?matchArms \<noteq> []" by simp
       have pats_compat: "list_all (\<lambda>p. pattern_compatible ?env' p CoreTy_Bool) (map fst ?matchArms)"
         by simp
-      have pats_regular: "patterns_regular (map fst ?matchArms)"
-        by (simp add: patterns_regular_def)
       have bodies_typed: "list_all (\<lambda>body. core_term_type ?env' ghost body = Some ?resultTy) (map snd ?matchArms)"
         using then'_typed else'_typed by simp
       show ?thesis
-        using finalCond_typed \<open>?matchArms \<noteq> []\<close> pats_compat pats_regular bodies_typed
+        using finalCond_typed \<open>?matchArms \<noteq> []\<close> pats_compat bodies_typed
         by (simp add: then'_typed)
     qed
     thus ?thesis using result_eq by simp
@@ -2382,12 +2380,10 @@ next
       have "?matchArms \<noteq> []" by simp
       have pats_compat: "list_all (\<lambda>p. pattern_compatible ?env' p CoreTy_Bool) (map fst ?matchArms)"
         by simp
-      have pats_regular: "patterns_regular (map fst ?matchArms)"
-        by (simp add: patterns_regular_def)
       have bodies_typed: "list_all (\<lambda>body. core_term_type ?env' ghost body = Some commonTy) (map snd ?matchArms)"
         using coerced_then_typed coerced_else_typed by simp
       show ?thesis
-        using finalCond_typed \<open>?matchArms \<noteq> []\<close> pats_compat pats_regular bodies_typed
+        using finalCond_typed \<open>?matchArms \<noteq> []\<close> pats_compat bodies_typed
         by (simp add: coerced_then_typed)
     qed
     thus ?thesis using result_eq by simp
